chore(library/init): cleanup proofs using new elaborator

library/init/wf.lean
@@ -8,69 +8,64 @@ import init.relation init.nat init.prod
 
 universe variables u v
 
-inductive acc {A : Type u} (R : A → A → Prop) : A → Prop
-| intro : ∀ x, (∀ y, R y x → acc y) → acc x
+inductive acc {A : Type u} (r : A → A → Prop) : A → Prop
+| intro : ∀ x, (∀ y, r y x → acc y) → acc x
 
 namespace acc
-  variables {A : Type u} {R : A → A → Prop}
+  variables {A : Type u} {r : A → A → Prop}
 
-  definition inv {x y : A} (H₁ : acc R x) (H₂ : R y x) : acc R y :=
-  acc.rec_on H₁ (λ x₁ ac₁ iH H₂, ac₁ y H₂) H₂
+  definition inv {x y : A} (h₁ : acc r x) (h₂ : r y x) : acc r y :=
+  acc.rec_on h₁ (λ x₁ ac₁ ih h₂, ac₁ y h₂) h₂
 
   -- dependent elimination for acc
   attribute [recursor]
   protected definition drec
-      {C : Π (a : A), acc R a → Type v}
-      (h₁ : Π (x : A) (acx : Π (y : A), R y x → acc R y),
-              (Π (y : A) (ryx : R y x), C y (acx y ryx)) → C x (acc.intro x acx))
-      {a : A} (h₂ : acc R a) : C a h₂ :=
-  @acc.rec _ _ (λ (a : A), Π (x : @acc A R a), C a x)
-    (λ x acx ih h₂, h₁ x acx (λ y ryx, ih y ryx (acx y ryx)))
-    _
-    h₂
-    h₂
+      {C : Π (a : A), acc r a → Type v}
+      (h₁ : Π (x : A) (acx : Π (y : A), r y x → acc r y), (Π (y : A) (ryx : r y x), C y (acx y ryx)) → C x (acc.intro x acx))
+      {a : A} (h₂ : acc r a) : C a h₂ :=
+  acc.rec (λ x acx ih h₂, h₁ x acx (λ y ryx, ih y ryx (acx y ryx))) h₂ h₂
 end acc
 
-inductive well_founded {A : Type u} (R : A → A → Prop) : Prop
-| intro : (∀ a, acc R a) → well_founded
+inductive well_founded {A : Type u} (r : A → A → Prop) : Prop
+| intro : (∀ a, acc r a) → well_founded
 
 namespace well_founded
-  definition apply {A : Type u} {R : A → A → Prop} (wf : well_founded R) : ∀ a, acc R a :=
+  definition apply {A : Type u} {r : A → A → Prop} (wf : well_founded r) : ∀ a, acc r a :=
   take a, well_founded.rec_on wf (λ p, p) a
 
   section
-  parameters {A : Type u} {R : A → A → Prop}
-  local infix `≺`:50    := R
+  parameters {A : Type u} {r : A → A → Prop}
+  local infix `≺`:50    := r
 
-  hypothesis Hwf : well_founded R
+  hypothesis hwf : well_founded r
 
-  theorem recursion {C : A → Type v} (a : A) (H : Π x, (Π y, y ≺ x → C y) → C x) : C a :=
-  acc.rec_on (apply Hwf a) (λ x₁ ac₁ iH, H x₁ iH)
+  theorem recursion {C : A → Type v} (a : A) (h : Π x, (Π y, y ≺ x → C y) → C x) : C a :=
+  acc.rec_on (apply hwf a) (λ x₁ ac₁ ih, h x₁ ih)
 
-  theorem induction {C : A → Prop} (a : A) (H : ∀ x, (∀ y, y ≺ x → C y) → C x) : C a :=
-  recursion a H
+  theorem induction {C : A → Prop} (a : A) (h : ∀ x, (∀ y, y ≺ x → C y) → C x) : C a :=
+  recursion a h
 
   variable {C : A → Type v}
   variable F : Π x, (Π y, y ≺ x → C y) → C x
 
-  definition fix_F (x : A) (a : acc R x) : C x :=
-  acc.rec_on a (λ x₁ ac₁ iH, F x₁ iH)
+  definition fix_F (x : A) (a : acc r x) : C x :=
+  acc.rec_on a (λ x₁ ac₁ ih, F x₁ ih)
 
-  theorem fix_F_eq (x : A) (r : acc R x) :
+  theorem fix_F_eq (x : A) (r : acc r x) :
     fix_F F x r = F x (λ (y : A) (p : y ≺ x), fix_F F y (acc.inv r p)) :=
   acc.drec (λ x r ih, rfl) r
   end
 
-  variables {A : Type u} {C : A → Type v} {R : A → A → Prop}
+  variables {A : Type u} {C : A → Type v} {r : A → A → Prop}
 
   -- Well-founded fixpoint
-  definition fix (Hwf : well_founded R) (F : Π x, (Π y, R y x → C y) → C x) (x : A) : C x :=
-  fix_F F x (apply Hwf x)
+  definition fix (hwf : well_founded r) (F : Π x, (Π y, r y x → C y) → C x) (x : A) : C x :=
+  fix_F F x (apply hwf x)
 
   -- Well-founded fixpoint satisfies fixpoint equation
-  theorem fix_eq (Hwf : well_founded R) (F : Π x, (Π y, R y x → C y) → C x) (x : A) :
-    fix Hwf F x = F x (λ y h, fix Hwf F y) :=
-  fix_F_eq F x (apply Hwf x)
+  theorem fix_eq (hwf : well_founded r) (F : Π x, (Π y, r y x → C y) → C x) (x : A) :
+    fix hwf F x = F x (λ y h, fix hwf F y) :=
+  fix_F_eq F x (apply hwf x)
 end well_founded
 
 open well_founded
@@ -83,95 +78,64 @@ well_founded.intro (λ (a : A),
 -- Subrelation of a well-founded relation is well-founded
 namespace subrelation
 section
-  parameters {A : Type u} {R Q : A → A → Prop}
-  parameters (H₁ : subrelation Q R)
-  parameters (H₂ : well_founded R)
+  parameters {A : Type u} {r Q : A → A → Prop}
+  parameters (h₁ : subrelation Q r)
+  parameters (h₂ : well_founded r)
 
-  definition accessible {a : A} (ac : acc R a) : acc Q a :=
+  definition accessible {a : A} (ac : acc r a) : acc Q a :=
   acc.rec_on ac (λ x ax ih,
-    acc.intro x (λ (y : A) (lt : Q y x), ih y (H₁ lt)))
+    acc.intro x (λ (y : A) (lt : Q y x), ih y (h₁ lt)))
 
   definition wf : well_founded Q :=
-  well_founded.intro (λ a, accessible (apply H₂ a))
+  ⟨λ a, accessible (apply h₂ a)⟩
 end
 end subrelation
 
 -- The inverse image of a well-founded relation is well-founded
 namespace inv_image
 section
-  parameters {A : Type u} {B : Type v} {R : B → B → Prop}
+  parameters {A : Type u} {B : Type v} {r : B → B → Prop}
   parameters (f : A → B)
-  parameters (H : well_founded R)
+  parameters (h : well_founded r)
 
-  private definition acc_aux : ∀ {b : B}, @acc B R b → (∀ (x : A), @eq B (f x) b → @acc A (@inv_image A B R f) x) :=
-  @acc.rec B R (λ (b : B), ∀ (x : A), f x = b → acc (inv_image R f) x)
-    (λ (x : B)
-       (acx : ∀ (y : B), R y x → acc R y)
-       (ih : ∀ (y : B), R y x → (λ (b : B), ∀ (x : A), f x = b → acc (inv_image R f) x) y)
-       (z : A) (e : f z = x),
-       acc.intro z
-         (λ (y : A) (lt : inv_image R f y z),
-            @eq.rec B (f z)
-              (λ (x : B),
-                 (∀ (y : B), R y x → acc R y) →
-                 (∀ (y : B), R y x → (λ (b : B), ∀ (x : A), f x = b → acc (inv_image R f) x) y) → acc (inv_image R f) y)
-              (λ (acx : ∀ (y : B), R y (f z) → @acc B R y)
-                 (ih :  ∀ (y : B), R y (f z) → (λ (b : B), ∀ (x : A), f x = b → acc (inv_image R f) x) y),
-                 ih (f y) lt y (@rfl B (f y)))
-              x
-              e
-              acx
-              ih))
+  private definition acc_aux {b : B} (ac : acc r b) : ∀ (x : A), f x = b → acc (inv_image r f) x :=
+  acc.rec_on ac (λ x acx ih z e,
+    acc.intro z (λ y lt, eq.rec_on e (λ acx ih, ih (f y) lt y rfl) acx ih))
 
-  definition accessible {a : A} (ac : acc R (f a)) : acc (inv_image R f) a :=
+  definition accessible {a : A} (ac : acc r (f a)) : acc (inv_image r f) a :=
   acc_aux ac a rfl
 
-  definition wf : well_founded (inv_image R f) :=
-  well_founded.intro (λ a, accessible (apply H (f a)))
+  definition wf : well_founded (inv_image r f) :=
+  ⟨λ a, accessible (apply h (f a))⟩
 end
 end inv_image
 
 -- The transitive closure of a well-founded relation is well-founded
 namespace tc
 section
-  parameters {A : Type u} {R : A → A → Prop}
-  local notation `R⁺` := tc R
+  parameters {A : Type u} {r : A → A → Prop}
+  local notation `r⁺` := tc r
 
-  definition accessible : ∀ {z : A}, acc R z → acc (tc R) z :=
-  @acc.rec A R (acc (tc R))
-    (λ (x : A) (acx : ∀ (y : A), R y x → acc R y) (ih : ∀ (y : A), R y x → acc (tc R) y),
-       @acc.intro A (tc R) x
-         (λ (y : A) (rel : tc R y x),
-            @tc.rec A R
-              (λ (y x : A),
-                 (∀ (y : A), R y x → acc R y) →
-                 (∀ (y : A), R y x → acc (tc R) y) → acc (tc R) y)
-              (λ (a b : A) (rab : R a b) (acx : ∀ (y : A), R y b → acc R y)
-                 (ih : ∀ (y : A), R y b → acc (tc R) y),
-                 ih a rab)
-              (λ (a b c : A) (rab : tc R a b) (rbc : tc R b c)
-                 (ih₁ : (∀ (y : A), R y b → acc R y) → (∀ (y : A), R y b → acc (tc R) y) → acc (tc R) a)
-                 (ih₂ : (∀ (y : A), R y c → acc R y) → (∀ (y : A), R y c → acc (tc R) y) → acc (tc R) b)
-                 (acx : ∀ (y : A), R y c → acc R y) (ih : ∀ (y : A), R y c → acc (tc R) y),
-                 @acc.inv A (@tc A R) b a (ih₂ acx ih) rab)
-              y
-              x
-              rel
-              acx
-              ih))
+  definition accessible {z : A} (ac : acc r z) : acc (tc r) z :=
+  acc.rec_on ac (λ x acx ih,
+    acc.intro x (λ y rel,
+      tc.rec_on rel
+        (λ a b rab acx ih, ih a rab)
+        (λ a b c rab rbc ih₁ ih₂ acx ih, acc.inv (ih₂ acx ih) rab)
+        acx ih))
 
-  definition wf (H : well_founded R) : well_founded R⁺ :=
-  well_founded.intro (λ a, accessible (apply H a))
+  definition wf (h : well_founded r) : well_founded r⁺ :=
+  ⟨λ a, accessible (apply h a)⟩
 end
 end tc
 
 -- less-than is well-founded
 definition nat.lt_wf : well_founded nat.lt :=
-well_founded.intro (nat.rec
-  (acc.intro 0 (λ n H, absurd H (nat.not_lt_zero n)))
-  (λ n IH, acc.intro (nat.succ n) (λ m H,
-     or.elim (nat.eq_or_lt_of_le (nat.le_of_succ_le_succ H))
-        (λ e, eq.substr e IH) (acc.inv IH))))
+⟨nat.rec
+  (acc.intro 0 (λ n h, absurd h (nat.not_lt_zero n)))
+  (λ n ih, acc.intro (nat.succ n) (λ m h,
+     or.elim (nat.eq_or_lt_of_le (nat.le_of_succ_le_succ h))
+        (λ e, eq.substr e ih) (acc.inv ih)))⟩
 
 definition measure {A : Type u} : (A → ℕ) → A → A → Prop :=
 inv_image lt
@@ -184,56 +148,46 @@ namespace prod
 
   section
   variables {A : Type u} {B : Type v}
-  variable  (Ra  : A → A → Prop)
-  variable  (Rb  : B → B → Prop)
+  variable  (ra  : A → A → Prop)
+  variable  (rb  : B → B → Prop)
 
-  -- Lexicographical order based on Ra and Rb
+  -- Lexicographical order based on ra and rb
   inductive lex : A × B → A × B → Prop
-  | left  : ∀ {a₁ b₁} a₂ b₂, Ra a₁ a₂ → lex (a₁, b₁) (a₂, b₂)
-  | right : ∀ a {b₁ b₂},     Rb b₁ b₂ → lex (a, b₁)  (a, b₂)
+  | left  : ∀ {a₁ b₁} a₂ b₂, ra a₁ a₂ → lex (a₁, b₁) (a₂, b₂)
+  | right : ∀ a {b₁ b₂},     rb b₁ b₂ → lex (a, b₁)  (a, b₂)
 
-  -- Relational product based on Ra and Rb
+  -- relational product based on ra and rb
   inductive rprod : A × B → A × B → Prop
-  | intro : ∀ {a₁ b₁ a₂ b₂}, Ra a₁ a₂ → Rb b₁ b₂ → rprod (a₁, b₁) (a₂, b₂)
+  | intro : ∀ {a₁ b₁ a₂ b₂}, ra a₁ a₂ → rb b₁ b₂ → rprod (a₁, b₁) (a₂, b₂)
   end
 
   section
   parameters {A : Type u} {B : Type v}
-  parameters {Ra  : A → A → Prop} {Rb  : B → B → Prop}
-  local infix `≺`:50 := lex Ra Rb
+  parameters {ra  : A → A → Prop} {rb  : B → B → Prop}
+  local infix `≺`:50 := lex ra rb
 
-  definition lex_accessible {a} (aca : acc Ra a) (acb : ∀ b, acc Rb b): ∀ b, acc (lex Ra Rb) (a, b) :=
-  acc.rec_on aca
-    (λ xa aca (iHa : ∀ y, Ra y xa → ∀ b, acc (lex Ra Rb) (y, b)),
-      λ b, acc.rec_on (acb b)
-        (λ xb acb
-          (iHb : ∀ y, Rb y xb → acc (lex Ra Rb) (xa, y)),
-          acc.intro (xa, xb) (λ p (lt : p ≺ (xa, xb)),
-            have aux : xa = xa → xb = xb → acc (lex Ra Rb) p, from
-              @prod.lex.rec_on A B Ra Rb (λ p₁ p₂, fst p₂ = xa → snd p₂ = xb → acc (lex Ra Rb) p₁)
-                               p (xa, xb) lt
-                (λ a₁ b₁ a₂ b₂ (H : Ra a₁ a₂) (eq₂ : a₂ = xa) (eq₃ : b₂ = xb),
-                  show acc (lex Ra Rb) (a₁, b₁), from
-                  have Ra₁  : Ra a₁ xa, from eq.rec_on eq₂ H,
-                  iHa a₁ Ra₁ b₁)
-                (λ a b₁ b₂ (H : Rb b₁ b₂) (eq₂ : a = xa) (eq₃ : b₂ = xb),
-                  show acc (lex Ra Rb) (a, b₁), from
-                  have Rb₁  : Rb b₁ xb, from eq.rec_on eq₃ H,
-                  have eq₂' : xa = a, from eq.rec_on eq₂ rfl,
-                  eq.rec_on eq₂' (iHb b₁ Rb₁)),
-            aux rfl rfl)))
+  definition lex_accessible {a} (aca : acc ra a) (acb : ∀ b, acc rb b): ∀ b, acc (lex ra rb) (a, b) :=
+  acc.rec_on aca (λ xa aca iha b,
+    acc.rec_on (acb b) (λ xb acb ihb,
+      acc.intro (xa, xb) (λ p lt,
+        have aux : xa = xa → xb = xb → acc (lex ra rb) p, from
+          @prod.lex.rec_on A B ra rb (λ p₁ p₂, fst p₂ = xa → snd p₂ = xb → acc (lex ra rb) p₁)
+                           p (xa, xb) lt
+            (λ a₁ b₁ a₂ b₂ h (eq₂ : a₂ = xa) (eq₃ : b₂ = xb), iha a₁ (eq.rec_on eq₂ h) b₁)
+            (λ a b₁ b₂ h (eq₂ : a = xa) (eq₃ : b₂ = xb), eq.rec_on eq₂~>symm (ihb b₁ (eq.rec_on eq₃ h))),
+        aux rfl rfl)))
 
   -- The lexicographical order of well founded relations is well-founded
-  definition lex_wf (Ha : well_founded Ra) (Hb : well_founded Rb) : well_founded (lex Ra Rb) :=
-  well_founded.intro (λ p, destruct p (λ a b, lex_accessible (apply Ha a) (well_founded.apply Hb) b))
+  definition lex_wf (ha : well_founded ra) (hb : well_founded rb) : well_founded (lex ra rb) :=
+  ⟨λ p, destruct p (λ a b, lex_accessible (apply ha a) (well_founded.apply hb) b)⟩
 
-  -- Relational product is a subrelation of the lex
-  definition rprod_sub_lex : ∀ a b, rprod Ra Rb a b → lex Ra Rb a b :=
-  λ a b H, prod.rprod.rec_on H (λ a₁ b₁ a₂ b₂ H₁ H₂, lex.left Rb a₂ b₂ H₁)
+  -- relational product is a subrelation of the lex
+  definition rprod_sub_lex : ∀ a b, rprod ra rb a b → lex ra rb a b :=
+  λ a b h, prod.rprod.rec_on h (λ a₁ b₁ a₂ b₂ h₁ h₂, lex.left rb a₂ b₂ h₁)
 
   -- The relational product of well founded relations is well-founded
-  definition rprod_wf (Ha : well_founded Ra) (Hb : well_founded Rb) : well_founded (rprod Ra Rb) :=
-  subrelation.wf (rprod_sub_lex) (lex_wf Ha Hb)
+  definition rprod_wf (ha : well_founded ra) (hb : well_founded rb) : well_founded (rprod ra rb) :=
+  subrelation.wf (rprod_sub_lex) (lex_wf ha hb)
 
   end
 
